Add proof for total correcness for loops

Com.v
@@ -7,22 +7,27 @@ From Rela Require Import Proc.
 From Rela Require Import Sigma.
 From Coq Require Import Lia.
 From Coq Require Import Lists.List.
+
 Import ListNotations.
 
 (** Definition of assertion **)
 
 Definition assertion : Type := list sigma -> Prop.
 
+(** Definition of variant **)
+
+Definition variant : Type := sigma -> nat .
+
 (** Defintion of command and program **)
 
 Inductive com : Type :=
 | CSkip
-| CAss (x : Loc.t) (a : aexp)
+| CAss (x : Loc.t) (a: aexp)
 | CAssr (x : Loc.t) (a : aexp)
 | CAssert (b: assertion )
 | CSeq (p1 : com) (p2 : com)
 | CIf (b : bexp) (p1 p2 : com)
-| CWhile (b : bexp) (p : com) (inv : assertion)
+| CWhile (b : bexp) (p : com) (inv : assertion) (var : variant)
 | CCall (f: Proc.t).
 
 (** Definition of procedure environment :
@@ -60,14 +65,14 @@ Inductive ceval : com -> sigma -> Psi.psi -> sigma -> Prop :=
       ceval p1 s ps s' ->
       ceval p2 s' ps s'' ->
       ceval (CSeq p1 p2) s ps s''
-  | E_WhileFalse : forall b s ps p inv,
+  | E_WhileFalse : forall b s ps p inv var,
       beval s b = false ->
-      ceval (CWhile b p inv) s  ps s
-  | E_WhileTrue : forall b s s' s'' ps p inv,
+      ceval (CWhile b p inv var) s  ps s
+  | E_WhileTrue : forall b s s' s'' ps p inv var,
       beval s b = true ->
       ceval p s ps s' ->
-      ceval (CWhile b p inv) s' ps s'' ->
-      ceval (CWhile b p inv) s  ps s''
+      ceval (CWhile b p inv var) s' ps s'' ->
+      ceval (CWhile b p inv var) s  ps s''
   | E_Call : forall s s' f ps,
       ceval ( ps f) s ps s' ->
       ceval (CCall f) s  ps s'
@@ -75,11 +80,11 @@ Inductive ceval : com -> sigma -> Psi.psi -> sigma -> Prop :=
 
 (** Facts about ceval **)
 
-Lemma ceval_inf_loop s ps s' :
-ceval (CWhile BTrue CSkip (fun _ => True)) s ps s' -> False.
+Lemma ceval_inf_loop s ps s' inv var :
+ceval (CWhile BTrue CSkip inv var) s ps s' -> False.
 Proof.
   intros Heval.
-  remember (CWhile BTrue CSkip (fun _ : list Sigma.sigma => True)) as original_command eqn:Horig.
+  remember (CWhile BTrue CSkip inv var) as original_command eqn:Horig.
   induction Heval;inversion Horig.
   * inversion Horig;subst. inversion H.
   * inversion Horig;subst.
@@ -89,198 +94,31 @@ Qed.
 Lemma ceval_det s ps c:
   forall s1' s2', ceval c s ps s1' -> ceval c s ps s2' -> s1' = s2'.
 Proof.
-  intros.
+  intros s1' s2' E1 E2.
   generalize dependent s2'.
-  induction H; intros st2 E2; inversion E2; subst.
+  induction E1; intros st2' E2 ; inversion E2; subst.
   - reflexivity.
   - reflexivity.
   - reflexivity.
   - reflexivity.
-  -  apply (IHceval _  H8).
+  - eapply IHE1; auto.
+  - rewrite H in H6.
+    discriminate H6.
+  - rewrite H in H6.
+    discriminate H6.
+  - eapply IHE1; auto.
+  - specialize (IHE1_1 s'0 H1).
+    subst.
+    apply (IHE1_2 _ H5).
+  - reflexivity.
   - rewrite H in H7.
     discriminate H7.
   - rewrite H in H7.
     discriminate H7.
-  - apply (IHceval _ H8).
-  - specialize (IHceval1 s'0 H3).
+  - specialize (IHE1_1 s'0 H8).
     subst.
-    apply (IHceval2 _ H7).
-  - reflexivity.
-  - rewrite H in H3.
-    discriminate H3.
-  - rewrite H in H8.
-    discriminate H8.
-  - specialize (IHceval1 s'0 H9).
-    subst.
-    apply (IHceval2 _ H10).
-  - apply (IHceval _ H1).
-Qed.
-
-(** Evaluation function for command **)
-
-Fixpoint ceval_step (s : sigma) (c : com) (i : nat) (ps : Psi.psi)
-                    : option sigma :=
-  match i with
-  | 0 => None
-  | S i' =>
-    match c with
-      | CSkip => Some s
-      | CAss x a => Some (x !-> aeval s a ; s)
-      | CAssr x a => Some ((s x) !-> aeval s a ; s)
-      | CAssert b => Some s
-      | CSeq c1 c2 =>
-          match (ceval_step s c1 i' ps) with
-          | Some s' => ceval_step s' c2 i' ps
-          | None => None
-          end
-      | CIf b c1 c2 =>
-          if (beval s b)
-            then ceval_step s c1 i' ps
-            else ceval_step s c2 i' ps
-      | CWhile b1 c1 inv =>
-          if (beval s b1)
-          then match (ceval_step s c1 i' ps) with
-               | Some s' => ceval_step s' c i' ps
-               | None => None
-               end
-          else Some s
-      | CCall f => ceval_step s (ps f) i' ps
-    end
-  end.
-
-(** Facts about ceval_step **)
-
-Lemma ceval_step_ceval: forall c s s' ps,
-      (exists i, ceval_step s c i ps = Some s') -> ceval c s ps s'.
-Proof.
-  intros.
-  destruct H.
-  generalize dependent s.
-  generalize dependent s'.
-  generalize  dependent c.
-  induction x; intros.
-  + simpl in H.
-    discriminate H.
-  + destruct c.
-  * inversion H. apply E_Skip.
-  * inversion H. apply E_Ass. reflexivity.
-  * inversion H. apply E_Assr. reflexivity.
-  * inversion H. apply E_Assert.
-  *  inversion H.
-    destruct (ceval_step s c1 x ps) eqn: H2.
-    - eapply E_Seq.
-      apply IHx. apply H2.
-      apply IHx. apply H1.
-    - discriminate H1.
-* inversion H.
-  destruct (beval s b) eqn: Hb.
-    - apply (E_IfTrue _ _ _ _ _ _ Hb).
-      apply IHx. apply H1.
-    - apply (E_IfFalse _ _ _ _ _ _ Hb).
-      apply IHx. apply H1.
-* inversion H.
-  destruct (beval s b) eqn: Hb.
-  - destruct (ceval_step s c x ps) eqn: Hcevalstep.
-    ++ apply (E_WhileTrue _ s s0 _ _ _ _ Hb).
-       apply IHx. apply Hcevalstep.
-       apply IHx. apply H1.
-    ++ discriminate H1.
-  - inversion H1. rewrite <- H2.
-    apply (E_WhileFalse _ _ _ _ _ Hb).
-* inversion H. apply E_Call. apply IHx.  apply H1.
-Qed.
-
-Lemma ceval_step_more: forall i1 i2 s s' c ps,
-  i1 <= i2 ->
-  ceval_step s c i1 ps = Some s' ->
-  ceval_step s c i2 ps = Some s'.
-Proof.
-induction i1 as [|i1']; intros i2 s s' c ps Hle Hceval.
-  - simpl in Hceval. discriminate Hceval.
-  - destruct i2 as [|i2']. inversion Hle.
-    assert (Hle': i1' <= i2') by lia.
-    destruct c.
-    +  simpl in Hceval. inversion Hceval.
-      reflexivity.
-    + simpl in Hceval. inversion Hceval.
-      reflexivity.
-    + simpl in Hceval. inversion Hceval.
-      reflexivity.
-    + simpl in Hceval. inversion Hceval.
-      reflexivity.
-    + simpl in Hceval. simpl.
-      destruct (ceval_step s c1 i1') eqn:Hcevalstep.
-      * rewrite (IHi1' _ _ _ _ _ Hle' Hcevalstep).
-        apply (IHi1' _ _ _ _ _ Hle' Hceval).
-      * discriminate Hceval.
-    + simpl. simpl in Hceval.
-      destruct (beval s b).
-      * apply (IHi1' _ _ _ _ _ Hle' Hceval).
-      * apply (IHi1' _ _ _ _ _ Hle' Hceval).
-    + simpl in Hceval. simpl.
-      destruct (beval s b).
-      * destruct (ceval_step s c i1') eqn: Hcevalstep.
-        -- rewrite (IHi1' _ _ _ _ _ Hle' Hcevalstep).
-           apply (IHi1' _ _ _ _ _ Hle' Hceval).
-        -- discriminate Hceval.
-      * assumption.
-    + simpl. simpl in Hceval.
-      apply (IHi1' _ _ _ _ _ Hle' Hceval).
-Qed.
-
-Lemma ceval_ceval_step: forall c s s' ps,
-      ceval c s ps s'  ->
-      exists i, ceval_step s c i ps = Some s'.
-Proof.
-  intros c s s' pc Hce.
-  induction Hce.
-  * exists 1. reflexivity.
-  * exists 1. simpl. rewrite H. reflexivity.
-  * exists 1. simpl. rewrite H. reflexivity.
-  * exists 1. simpl. reflexivity.
-  * destruct IHHce. exists (S x).
-    simpl. rewrite H. assumption.
-  * destruct IHHce. exists (S x).
-    simpl. rewrite H. assumption.
-  * destruct IHHce1.  destruct IHHce2.
-    exists (S (x + x0)). simpl.
-    destruct (ceval_step s p1 (x + x0) ps) eqn: Hceval_step.
-  - apply (ceval_step_more x0);[lia |].
-    apply (ceval_step_more _ (x + x0)) in H;[|lia].
-    rewrite H in Hceval_step.
-    inversion Hceval_step.
-    rewrite <- H2.
-    assumption.
-  - apply (ceval_step_more _ (x + x0)) in H;[|lia].
-    rewrite H in Hceval_step.
-    discriminate Hceval_step.
-  * exists 1. simpl. rewrite H. reflexivity.
-  * destruct IHHce1.
-    destruct IHHce2.
-    exists (S (x + x0)). simpl.
-    destruct (beval s b).
-    + destruct (ceval_step s p (x + x0) ps) eqn : Hcval_step.
-      - apply (ceval_step_more x0);[lia|].
-        apply (ceval_step_more _ (x + x0)) in H0;[| lia].
-        rewrite H0 in Hcval_step.
-        inversion Hcval_step. rewrite <- H3.
-        assumption.
-      - apply (ceval_step_more _ (x + x0)) in H0;[| lia].
-        rewrite H0 in Hcval_step.
-        discriminate Hcval_step.
-   + discriminate H.
-  * destruct IHHce.
-    exists (S x). simpl.
-    assumption.
-Qed.
-
-(** Both evaluation are equivalent **)
-
-Theorem ceval_and_ceval_step_coincide: forall c s s' ps,
-            ceval c s ps s' <-> exists i, ceval_step s c i ps = Some s'.
-Proof.
-  intros c s s' ps.
-  split. apply ceval_ceval_step. apply ceval_step_ceval.
+    apply (IHE1_2 _ H9).
+  - apply (IHE1 _ H0).
 Qed.
 
 (** Notations for program **)
